\appendix 

\section{Mathematical Symbols}

\begin{tabular}{|c|c|}
	\hline
	Name & Symbol \\
	\hline
	\hline
	\verb|Functor| & \hfe \\
	\hline
	\verb|Applicative| & \hayin \\
	\hline
	\verb|Monad| & \hmem \\
	\hline
	\verb|MonadTrans| & \htet \\
	\hline
	\verb|Foldable|\footnote{Catamorphism} & \hkaf \\
	\hline
	\verb|Traversable| & \htav \\
	\hline
	\verb|Semigroup| & \hsamekh \\
	\hline 
	\verb|MStep| & \hnun \\
	\hline 
	\verb|ChoiceT|\footnote{See Semetic "bhr"} & \hbet \\
	\hline
\end{tabular}
\section{Omitted Proofs}

\begin{lem}
	$\hfe \alpha \Rightarrow \hfe (\hnun \alpha)$
\end{lem}
\begin{proof}
	By elimination we transform to $\prove (f : \beta \to \gamma) \to (x : \hnun \beta) \to (\hnun \gamma)$.
	By introduction we have $(f : \beta \to \gamma), (x : \hnun \beta) \prove (\hnun \gamma)$
	We preform induction on $x$ to yield two cases, $\verb|map|_0 : (f : \beta \to \gamma) \to ([] : \hnun \alpha \beta) \to (\hnun \alpha \gamma)$ and $\verb|map|_0 : (f : \beta \to \gamma) \to ([] : \hnun \alpha \beta) \to (\hnun \alpha \gamma)$
\end{proof}
\begin{thm}
	
\end{thm}
\begin{proof}
	
\end{proof}
